# baseURI: https://w3id.org/def/basicsemantics-owl
# imports: http://qudt.org/schema/qudt
# imports: http://qudt.org/vocab/quantitykind
# imports: http://qudt.org/vocab/unit
# imports: http://www.w3.org/2004/02/skos/core

@prefix : <https://w3id.org/def/basicsemantics-owl#> .
@prefix nta8035: <https://w3id.org/def/basicsemantics-owl#> .
@prefix owl: <http://www.w3.org/2002/07/owl#> .
@prefix quantitykind: <http://qudt.org/vocab/quantitykind/> .
@prefix qudt: <http://qudt.org/schema/qudt/> .
@prefix rdf: <http://www.w3.org/1999/02/22-rdf-syntax-ns#> .
@prefix rdfs: <http://www.w3.org/2000/01/rdf-schema#> .
@prefix skos: <http://www.w3.org/2004/02/skos/core#> .
@prefix unit: <http://qudt.org/vocab/unit/> .
@prefix xsd: <http://www.w3.org/2001/XMLSchema#> .

<https://w3id.org/def/basicsemantics-owl>
  a owl:Ontology ;
  owl:imports <http://qudt.org/schema/qudt> ;
  owl:imports <http://qudt.org/vocab/quantitykind> ;
  owl:imports <http://qudt.org/vocab/unit> ;
  owl:imports <http://www.w3.org/2004/02/skos/core> ;
.
nta8035:Activity
  a owl:Class ;
  rdfs:subClassOf owl:Thing ;
  rdfs:subClassOf [
      a owl:Restriction ;
      owl:allValuesFrom nta8035:Activity ;
      owl:onProperty nta8035:hasPart ;
    ] ;
  skos:definition "An activity is something possibly or actual happens in space and time" ;
  skos:example "Fluid pressure measurement, driving a car are examples of an <activity> " ;
  skos:prefLabel "activiteit"@nl ;
  skos:prefLabel "activity"@en ;
  skos:scopeNote "Process, function, human activity, machine activity, task, procedure, project are subclasses of <Activity>." ;
.
nta8035:AddressSystem
  a owl:Class ;
  rdfs:subClassOf nta8035:SpatialReferenceSystem ;
  skos:prefLabel "address system"@en ;
  skos:prefLabel "adressysteem"@nl ;
.
nta8035:CalenderSystem
  a owl:Class ;
  rdfs:subClassOf nta8035:TemporalReferenceSystem ;
  skos:prefLabel "calender system"@en ;
  skos:prefLabel "kalendersysteem"@nl ;
.
nta8035:CoordinateReferenceSystem
  a owl:Class ;
  rdfs:subClassOf nta8035:SpatialReferenceSystem ;
  skos:prefLabel "coordinaatreferentiesysteem"@nl ;
  skos:prefLabel "coordinate reference system"@en ;
.
nta8035:EnumerationType
  a owl:Class ;
  rdfs:subClassOf owl:Thing ;
  skos:definition "The superclass of all user-defined enumeration classes where the allowed enumeration items are individuals" ;
  skos:example "LoadLevelType being Low, Medium or High" ;
  skos:prefLabel "enumeratietype"@nl ;
  skos:prefLabel "enumeration type"@en ;
.
nta8035:Event
  a owl:Class ;
  rdfs:subClassOf owl:Thing ;
  skos:definition "A thing that happens or takes place and marks the beginning or ending of an activity or state" ;
  skos:example "The connection of power to pump P_101, the take-off of a aeroplane are examples of an <Event>. " ;
  skos:prefLabel "event"@en ;
  skos:prefLabel "gebeurtenis"@nl ;
  skos:scopeNote "Transition, cause, effect, risk, milestone, issue, accident, point in time are subclasses of <Event>." ;
.
nta8035:IndexKnownSpatialLocations
  a owl:Class ;
  rdfs:subClassOf nta8035:SpatialReferenceSystem ;
  skos:prefLabel "index bekende ruimtelijke plaatsen"@nl ;
  skos:prefLabel "index known spatial locations"@en ;
.
nta8035:InformationObject
  a owl:Class ;
  rdfs:subClassOf owl:Thing ;
  rdfs:subClassOf [
      a owl:Restriction ;
      owl:allValuesFrom nta8035:InformationObject ;
      owl:onProperty nta8035:hasPart ;
    ] ;
  skos:definition "Thing that is a whole of information on itself and has an own identity" ;
  skos:example "a file within a computer system, the PDF file with URI http://material-certificate/M-101-1234.pdf are examples of <InformationObject> " ;
  skos:prefLabel "informatieobject"@nl ;
  skos:prefLabel "information object"@en ;
  skos:scopeNote "Requirement, document, statement, E-mail, code, identifier are subclasses of <InformationObject> ." ;
.
nta8035:LinearReferenceSystem
  a owl:Class ;
  rdfs:subClassOf nta8035:SpatialReferenceSystem ;
  skos:prefLabel "lineair referentiesysteem"@nl ;
  skos:prefLabel "linear reference system"@en ;
.
nta8035:PhysicalObject
  a owl:Class ;
  rdfs:subClassOf owl:Thing ;
  rdfs:subClassOf [
      a owl:Restriction ;
      owl:allValuesFrom nta8035:PhysicalObject ;
      owl:onProperty nta8035:hasPart ;
    ] ;
  skos:definition "Is something that possibly or actually exists in space and time, perceivable through the senses" ;
  skos:example "Pump P_101, a single living organism are examples of a <PhysicalObject>" ;
  skos:prefLabel "fysiek object"@nl ;
  skos:prefLabel "physical object"@en ;
  skos:scopeNote "Artefact, matter, person, organisation, stream, connection are subclasses of <PhysicalObject>." ;
.
nta8035:QuantityValue
  a owl:Class ;
  rdfs:subClassOf owl:Thing ;
  rdfs:subClassOf [
      a owl:Restriction ;
      owl:onClass xsd:decimal ;
      owl:onProperty rdf:value ;
      owl:qualifiedCardinality "1"^^xsd:nonNegativeInteger ;
    ] ;
  skos:prefLabel "kwantiteitwaarde"@nl ;
  skos:prefLabel "quantity value"@en ;
.
nta8035:SpatialLocation
  a owl:Class ;
  rdfs:subClassOf owl:Thing ;
  skos:prefLabel "ruimtelocatie"@nl ;
  skos:prefLabel "spatial location"@en ;
.
nta8035:SpatialReference
  a owl:Class ;
  rdfs:subClassOf owl:Thing ;
  skos:prefLabel "ruimtereferentie"@nl ;
  skos:prefLabel "spatial reference"@en ;
.
nta8035:SpatialReferenceSystem
  a owl:Class ;
  rdfs:subClassOf owl:Thing ;
  skos:prefLabel "ruimtereferentiesysteem"@nl ;
  skos:prefLabel "spatial reference system"@en ;
.
nta8035:SpatialRegion
  a owl:Class ;
  rdfs:subClassOf owl:Thing ;
  skos:definition "Demarcated space" ;
  skos:example "an IFC BREP or GeoSPARQL geometry representing a physical space, as special case of a physical object, such as an office space, a construction area for a building, a maritime traffic zone within the Channel, a hazard zone within a plant or the loading gauge of a train are examples of a <SpatialRegion>" ;
  skos:prefLabel "ruimtelijk gebied"@nl ;
  skos:prefLabel "spatial region"@en ;
.
nta8035:State
  a owl:Class ;
  rdfs:subClassOf owl:Thing ;
  skos:definition "A particular condition that something is in during a specific period in time" ;
  skos:example "well-functioning of a car, the condition of an elevator of being un-safe are examples of a <State>" ;
  skos:prefLabel "state"@en ;
  skos:prefLabel "toestand"@nl ;
  skos:scopeNote "Condition, failure state, objective are subclasses of <State>." ;
.
nta8035:TemporalCoordinateReferenceSystem
  a owl:Class ;
  rdfs:subClassOf nta8035:TemporalReferenceSystem ;
  skos:prefLabel "temporal coordinate reference system"@en ;
  skos:prefLabel "tijdcoordinaatreferentiesysteem"@nl ;
.
nta8035:TemporalLocation
  a owl:Class ;
  rdfs:subClassOf owl:Thing ;
  skos:prefLabel "temporal location"@en ;
  skos:prefLabel "tijdlocatie"@nl ;
.
nta8035:TemporalReference
  a owl:Class ;
  rdfs:subClassOf owl:Thing ;
  skos:prefLabel "temporal reference"@en ;
  skos:prefLabel "tijdreferentie"@nl ;
.
nta8035:TemporalReferenceSystem
  a owl:Class ;
  skos:prefLabel "temporal reference system"@en ;
  skos:prefLabel "tijdreferentiesysteem"@nl ;
.
nta8035:TemporalRegion
  a owl:Class ;
  rdfs:subClassOf owl:Thing ;
  skos:definition "A length or portion of time" ;
  skos:example "week 12 in 2019, design stage of the Schiphol tunnel are examples of a <TemporalRegion>" ;
  skos:prefLabel "temporal region"@en ;
  skos:prefLabel "temporeel gebied"@nl ;
  skos:scopeNote "Week, day, life cycle stage are subclasses of <TemporalRegion>." ;
.
nta8035:abbreviation
  a owl:AnnotationProperty ;
  rdfs:range xsd:string ;
  rdfs:subPropertyOf skos:altLabel ;
  skos:prefLabel "abbreviation"@en ;
  skos:prefLabel "afkorting"@nl ;
.
nta8035:begins
  a owl:ObjectProperty ;
  rdfs:domain nta8035:Event ;
  rdfs:range nta8035:Activity ;
  skos:definition "Deze relatie geldt tussen een Gebeurtenis en een Toestand."@nl ;
  skos:definition "This relationship applies between an Event and a State."@en ;
  skos:example "De blikseminslag (gebeurtenis) is het begin van de bosbrand (toestand)."@nl ;
  skos:example "The lightning strike (event) is the start of the forest fire (state)."@en ;
  skos:prefLabel "begins"@en ;
  skos:prefLabel "begint"@nl ;
.
nta8035:describes
  a owl:ObjectProperty ;
  rdfs:domain nta8035:InformationObject ;
  rdfs:range [
      a owl:Class ;
      owl:unionOf (
          nta8035:PhysicalObject
          nta8035:Activity
          nta8035:Event
          nta8035:State
          nta8035:InformationObject
        ) ;
    ] ;
  skos:definition "Deze relatie geldt tussen een Informatie Object en een Fysiek Object, een Activiteit, een Gebeurtenis, een Toestand, een Tijdperiode, een Ruimtelijk Gebied of een ander Informatie Object."@nl ;
  skos:definition "This relationship applies between an Information Object and a Physical Object, an Activity, an Event, a State, a Time Period, a Spatial Region or another Information Object."@en ;
  skos:example "Neem de Ketelbrug. Daar is in de loop der tijden een waar dossier ontstaan van tekeningen, specificaties, rapporten, nota's, in analoge of in digitale vorm. Elk van deze documenten beschrijft de Ketelbrug en kan worden gezien als een instantie van een Informatie Object die de Ketelbrug beschrijft."@nl ;
  skos:example "Take the Ketel bridge. Over time, a dossier has been created of drawings, specifications, reports, invoices, in analogue or in digital form. Each of these documents describes the Ketelbrug and can be seen as an instance of an Information Object that describes the Ketelbrug. "@en ;
  skos:prefLabel "beschrijft"@nl ;
  skos:prefLabel "describes"@en ;
.
nta8035:ends
  a owl:ObjectProperty ;
  rdfs:domain nta8035:Event ;
  rdfs:range nta8035:Activity ;
  skos:definition "Deze relatie geldt tussen een Gebeurtenis en een Toestand."@nl ;
  skos:definition "This relationship applies between an Event and a State."@en ;
  skos:example "Het onweer (gebeurtenis) beeindigde het mooie weer (toestand)."@nl ;
  skos:example "The thunderstorm (event) ended the nice weather (state)."@en ;
  skos:prefLabel "beeindigt"@nl ;
  skos:prefLabel "ends"@en ;
.
nta8035:hasBoundary
  a owl:ObjectProperty ;
  rdfs:domain [
      a owl:Class ;
      owl:unionOf (
          nta8035:PhysicalObject
          nta8035:Activity
        ) ;
    ] ;
  rdfs:range nta8035:SpatialRegion ;
  skos:definition "Deze relatie geldt tussen een Fysiek Object en een Ruimtelijk Gebied."@nl ;
  skos:definition "This relationship applies between a Physical Object and a Spatial Region."@en ;
  skos:example "A parcel is bounded by a 1D GML polyline."@en ;
  skos:example "Een perceel wordt begrensd door een 1D GML polyline."@nl ;
  skos:prefLabel "has boundary"@en ;
  skos:prefLabel "heeft begrenzing"@nl ;
.
nta8035:hasInterior
  a owl:ObjectProperty ;
  rdfs:domain [
      a owl:Class ;
      owl:unionOf (
          nta8035:PhysicalObject
          nta8035:Activity
        ) ;
    ] ;
  rdfs:range nta8035:SpatialRegion ;
  skos:definition "Deze relatie geldt tussen een Fysiek Object en een (topologisch) Ruimtelijk Gebied, tussen een Activiteit en een Ruimtelijk Gebied en tussen een Toestand en een Ruimtelijk Gebied."@nl ;
  skos:definition "This relationship applies between a Physical Object and a (topological) Spatial Region, between an Activity and a Spatial Region and between a State and a Spatial Region."@en ;
  skos:example "An IfcSpace as physical space can have a Constructive Solid Geometry (CSG) representation as a special case of a 3D region in space."@nl ;
  skos:example "Een IfcSpace als fysieke ruimte kan een Constructive Solid Geometry (CSG) representatie hebben als speciaal geval van een 3D ruimtelijk gebied."@nl ;
  skos:prefLabel "has interior"@en ;
  skos:prefLabel "heeft inwendige"@nl ;
.
nta8035:hasPart
  a owl:ObjectProperty ;
  skos:definition "Deze relatie, zoals al generiek geintroduceerd in de CMM, geldt tussen Fysiek Objecten onderling, tussen Informatie Objecten onderling of tussen Activiteiten onderling."@nl ;
  skos:definition "This relationship, as already generically introduced in the CMM, applies between Physical Objects themselves, between Information Objects themselves or between Activities themselves."@en ;
  skos:example "De fiets van Ellen (fysiek object) bestaat uit een frame, twee wielen en diverse andere onderdelen (allen fysieke objecten)."@nl ;
  skos:example "Ellen's bicycle (physical object) consists of a frame, two wheels and various other parts (all physical objects)."@en ;
  skos:prefLabel "has part"@en ;
  skos:prefLabel "heeft deel"@nl ;
.
nta8035:hasPeriod
  a owl:ObjectProperty ;
  rdfs:domain [
      a owl:Class ;
      owl:unionOf (
          nta8035:PhysicalObject
          nta8035:Activity
        ) ;
    ] ;
  rdfs:range nta8035:TemporalRegion ;
  skos:definition "Deze relatie geldt tussen een Toestand en een Tijdperiode of tussen een Fysiek Object en een Tijdperiode."@nl ;
  skos:definition "This relationship applies between a Condition and a Time Period or between a Physical Object and a Time Period."@en ;
  skos:example "From Friday 26 July up to and including Sunday 18 August 2019 (time period) the N231 (physical object) is completely closed off (condition) due to major maintenance (activity)."@en ;
  skos:example "Van vrijdag 26 juli tot en met zondag 18 augustus 2019 (tijdperiode) is de N231 (fysiek object) volledig afgesloten (toestand) vanwege groot onderhoud (activiteit)."@nl ;
  skos:prefLabel "has period"@en ;
  skos:prefLabel "heeft periode"@nl ;
.
nta8035:hasSpatialLocation
  a owl:ObjectProperty ;
  rdfs:domain nta8035:SpatialRegion ;
  rdfs:range nta8035:SpatialLocation ;
  skos:prefLabel "has spatial location"@en ;
  skos:prefLabel "heeft ruimtelocatie"@nl ;
.
nta8035:hasSpatialReference
  a owl:ObjectProperty ;
  rdfs:domain nta8035:SpatialLocation ;
  rdfs:range nta8035:SpatialReference ;
  skos:prefLabel "has spatial reference"@en ;
  skos:prefLabel "heeft ruimtereferentie"@nl ;
.
nta8035:hasSpatialReferenceSystem
  a owl:ObjectProperty ;
  rdfs:domain nta8035:SpatialLocation ;
  rdfs:range nta8035:SpatialReferenceSystem ;
  skos:prefLabel "has spatial reference system"@en ;
  skos:prefLabel "heeft ruimtereferentiesysteem"@nl ;
.
nta8035:hasState
  a owl:ObjectProperty ;
  rdfs:domain [
      a owl:Class ;
      owl:unionOf (
          nta8035:PhysicalObject
          nta8035:Activity
        ) ;
    ] ;
  rdfs:range nta8035:State ;
  skos:definition "Deze relatie geldt tussen een Activiteit en een Toestand of tussen een Fysiek Object en een Toestand."@nl ;
  skos:definition "This relationship applies between an Activity and a State or between a Physical Object and a State."@en ;
  skos:example "A state can contain multiple parameters. In this way, the air pressure, temperature and humidity of a piece of atmosphere can be recorded. These three parameters then define the state of the atmosphere at a certain location and time."@en ;
  skos:example "Een toestand kan meerdere parameters bevatten. Zo kan van een stukje atmosfeer zowel de luchtdruk, temperatuur als de luchtvochtigheid worden vastgelegd. Deze drie parameters definieren dan de toestand van de atmosfeer op een bepaalde locatie en een bepaald tijdstip."@nl ;
  skos:prefLabel "has state"@en ;
  skos:prefLabel "heeft toestand"@nl ;
.
nta8035:hasTemporalLocation
  a owl:ObjectProperty ;
  rdfs:domain nta8035:TemporalRegion ;
  rdfs:range nta8035:TemporalLocation ;
  skos:prefLabel "has temporal location"@en ;
  skos:prefLabel "heeft tijdlocatie"@nl ;
.
nta8035:hasTemporalReference
  a owl:ObjectProperty ;
  rdfs:domain nta8035:TemporalLocation ;
  rdfs:range nta8035:TemporalReference ;
  skos:prefLabel "has temporal reference"@en ;
  skos:prefLabel "heeft tijdreferentie"@nl ;
.
nta8035:hasTemporalReferenceSystem
  a owl:ObjectProperty ;
  rdfs:domain nta8035:TemporalLocation ;
  rdfs:range nta8035:TemporalReferenceSystem ;
  skos:prefLabel "has temporal reference system"@en ;
  skos:prefLabel "heeft tijdreferentiesysteem"@nl ;
.
nta8035:performs
  a owl:ObjectProperty ;
  rdfs:domain nta8035:PhysicalObject ;
  rdfs:range nta8035:Activity ;
  skos:definition "Deze relatie geldt tussen een Fysiek Object en een Activiteit."@nl ;
  skos:definition "This relationship applies between a Physical Object and an Activity."@en ;
  skos:example "Het Lassen van een brugleuning (een activiteit) wordt uitgevoerd met behulp van een Lasapparaat (fysiek object) en de Lasser (fysiek object)."@nl ;
  skos:example "The welding of a bridge railing (an activity) is carried out with the aid of a welding machine (physical object) and the welder (physical object)."@en ;
  skos:prefLabel "performs"@en ;
  skos:prefLabel "voert uit"@nl ;
.
nta8035:quantityKind
  a owl:ObjectProperty ;
  rdfs:range qudt:QuantityKind ;
  skos:prefLabel "grootheid"@nl ;
  skos:prefLabel "quantity kind"@en ;
.
nta8035:transforms
  a owl:ObjectProperty ;
  rdfs:domain nta8035:Activity ;
  rdfs:range nta8035:PhysicalObject ;
  skos:definition "Deze relatie geldt tussen een Activiteit en een Fysiek Object of tussen een Activiteit en een Informatie Object."@nl ;
  skos:definition "This relationship applies between an Activity and a Physical Object or between an Activity and an Information Object."@en ;
  skos:example "Baking (an activity) transforms a pizza (a physical object) from unbaked (a state) to baked (another state)."@en ;
  skos:example "Het Bakken (een activiteit) transformeert een pizza (een fysiek object) van ongebakken (een toestand) naar gebakken (een andere toestand)."@nl ;
  skos:prefLabel "transformeert"@nl ;
  skos:prefLabel "transforms"@en ;
.
nta8035:triggers
  a owl:ObjectProperty ;
  rdfs:domain [
      a owl:Class ;
      owl:unionOf (
          nta8035:PhysicalObject
          nta8035:Activity
        ) ;
    ] ;
  rdfs:range nta8035:Event ;
  skos:definition "Deze relatie geldt tussen een Gebeurtenis en een Activiteit en een Gebeurtenis en een Fysiek Object."@nl ;
  skos:definition "This relationship applies between an Event and an Activity and an Event and a Physical Object."@en ;
  skos:example "Neem een Verkeersongeval (een gebeurtenis). Deze initieert de komst van de hulpdiensten (een activiteit)."@nl ;
  skos:example "Take a traffic accident (an event). This initiates the arrival of the emergency services (an activity)."@en ;
  skos:prefLabel "triggers"@en ;
  skos:prefLabel "triggert"@nl ;
.
nta8035:unit
  a owl:ObjectProperty ;
  rdfs:range qudt:Unit ;
  skos:prefLabel "eenheid"@nl ;
  skos:prefLabel "unit"@en ;
.
[
  a owl:AllDisjointClasses ;
  owl:members (
      nta8035:PhysicalObject
      nta8035:InformationObject
      nta8035:State
      nta8035:Event
      nta8035:TemporalRegion
      nta8035:SpatialRegion
      nta8035:Activity
    ) ;
].
